cont. rework: Basic FSM properties

Experiments/FSM.thy
@@ -745,7 +745,7 @@ lemma acyclic_paths_set :
   by (metis (no_types, lifting) One_nat_def Suc_pred cyclic_path_shortening leD list.size(3) not_less_eq_eq not_less_zero path.intros(1) path_begin_node) 
 
 
-
+(* inefficient calculation, as a node may be target of a large number of (acyclic) paths *)
 lemma reachable_nodes_code[code] : 
   "reachable_nodes M q = image (target (initial M)) (acyclic_paths_up_to_length M (initial M) (size M - 1))"
 proof -
@@ -772,6 +772,717 @@ proof -
     unfolding reachable_nodes_def acyclic_paths_set by blast
   ultimately show ?thesis by blast
 qed
+
+
+
+subsection \<open>Language\<close>
+
+abbreviation "p_io (p :: ('state,'input,'output) path) \<equiv> map (\<lambda> t . (t_input t, t_output t)) p"
+
+fun language_state_for_input :: "('state,'input,'output) fsm \<Rightarrow> 'state \<Rightarrow> 'input list \<Rightarrow> ('input \<times> 'output) list set" where
+  "language_state_for_input M q xs = {p_io p | p . path M q p \<and> map fst (p_io p) = xs}"
+
+fun LS\<^sub>i\<^sub>n :: "('state,'input,'output) fsm \<Rightarrow> 'state \<Rightarrow> 'input list set \<Rightarrow> ('input \<times> 'output) list set" where
+  "LS\<^sub>i\<^sub>n M q xss = {p_io p | p . path M q p \<and> map fst (p_io p) \<in> xss}"
+
+abbreviation(input) "L\<^sub>i\<^sub>n M \<equiv> LS\<^sub>i\<^sub>n M (initial M)"
+
+lemma language_state_for_input_inputs : 
+  assumes "io \<in> language_state_for_input M q xs"
+  shows "map fst io = xs" 
+  using assms by auto
+
+lemma language_state_for_inputs_inputs : 
+  assumes "io \<in> LS\<^sub>i\<^sub>n M q xss"
+  shows "map fst io \<in> xss" using assms by auto 
+
+
+fun LS :: "('state,'input,'output) fsm \<Rightarrow> 'state \<Rightarrow> ('input \<times> 'output) list set" where
+  "LS M q = { p_io p | p . path M q p }"
+
+abbreviation "L M \<equiv> LS M (initial M)"
+
+lemma language_state_containment :
+  assumes "path M q p"
+  and     "p_io p = io"
+shows "io \<in> LS M q"
+  using assms by auto
+
+lemma language_prefix : 
+  assumes "io1@io2 \<in> LS M q"
+  shows "io1 \<in> LS M q"
+proof -
+  obtain p where "path M q p" and "p_io p = io1@io2" 
+    using assms by auto
+  let ?tp = "take (length io1) p"
+  have "path M q ?tp"
+    by (metis (no_types) \<open>path M q p\<close> append_take_drop_id path_prefix) 
+  moreover have "p_io ?tp = io1"
+    using \<open>p_io p = io1@io2\<close> by (metis append_eq_conv_conj take_map) 
+  ultimately show ?thesis
+    by force 
+qed
+
+lemma language_contains_empty_sequence : "[] \<in> L M" by auto
+
+
+lemma language_state_split :
+  assumes "io1 @ io2 \<in> LS M q1"
+  obtains  p1 p2 where "path M q1 p1" and "path M (target q1 p1) p2"  and "p_io p1 = io1" and "p_io p2 = io2"
+proof -
+  obtain p12 where "path M q1 p12" and "p_io p12 = io1 @ io2"
+    using assms unfolding LS.simps by auto
+
+  let ?p1 = "take (length io1) p12"
+  let ?p2 = "drop (length io1) p12"
+
+  have "p12 = ?p1 @ ?p2" 
+    by auto
+  then have "path M q1 (?p1 @ ?p2)"
+    using \<open>path M q1 p12\<close> by auto
+
+  have "path M q1 ?p1" and "path M (target q1 ?p1) ?p2"
+    using path_append_elim[OF \<open>path M q1 (?p1 @ ?p2)\<close>] by blast+
+  moreover have "p_io ?p1 = io1"
+    using \<open>p12 = ?p1 @ ?p2\<close> \<open>p_io p12 = io1 @ io2\<close>
+    by (metis append_eq_conv_conj take_map)
+  moreover have "p_io ?p2 = io2"
+    using \<open>p12 = ?p1 @ ?p2\<close> \<open>p_io p12 = io1 @ io2\<close>
+    by (metis (no_types) \<open>p_io p12 = io1 @ io2\<close> append_eq_conv_conj drop_map) 
+  ultimately show ?thesis using that by blast
+qed
+
+
+
+
+
+
+subsection \<open> Basic FSM properties \<close>
+
+subsubsection \<open>Completely Specified\<close>
+
+fun completely_specified :: "('a,'b,'c) fsm \<Rightarrow> bool" where
+  "completely_specified M = (\<forall> q \<in> nodes M . \<forall> x \<in> inputs M . \<exists> t \<in> transitions M . t_source t = q \<and> t_input t = x)"
+
+
+lemma completely_specified_alt_def : "completely_specified M = (\<forall> q \<in> nodes M . \<forall> x \<in> inputs M . \<exists> q' y . (q,x,y,q') \<in> transitions M)"
+  by force
+
+lemma completely_specified_alt_def_h : "completely_specified M = (\<forall> q \<in> nodes M . \<forall> x \<in> inputs M . h M (q,x) \<noteq> {})"
+  by force
+
+
+value "completely_specified m_ex_H"
+
+
+
+fun completely_specified_state :: "('a,'b,'c) fsm \<Rightarrow> 'a \<Rightarrow> bool" where
+  "completely_specified_state M q = (\<forall> x \<in> inputs M . \<exists> t \<in> transitions M . t_source t = q \<and> t_input t = x)"
+
+lemma completely_specified_states :
+  "completely_specified M = (\<forall> q \<in> nodes M . completely_specified_state M q)"
+  unfolding completely_specified.simps completely_specified_state.simps by force
+
+lemma completely_specified_state_alt_def_h : "completely_specified_state M q = (\<forall> x \<in> inputs M . h M (q,x) \<noteq> {})"
+  by force
+
+
+subsubsection \<open>Deterministic\<close>
+
+fun deterministic :: "('a,'b,'c) fsm \<Rightarrow> bool" where
+  "deterministic M = (\<forall> t1 \<in> transitions M . \<forall> t2 \<in> transitions M . t_source t1 = t_source t2 \<and> t_input t1 = t_input t2 \<longrightarrow> t_output t1 = t_output t2 \<and> t_target t1 = t_target t2)" 
+
+lemma deterministic_alt_def : "deterministic M = (\<forall> q1 x y' y''  q1' q1'' . (q1,x,y',q1') \<in> transitions M \<and> (q1,x,y'',q1'') \<in> transitions M \<longrightarrow> y' = y'' \<and> q1' = q1'')" 
+  by auto
+
+lemma deterministic_alt_def_h : "deterministic M = (\<forall> q1 x yq yq' . (yq \<in> h M (q1,x) \<and> yq' \<in> h M (q1,x)) \<longrightarrow> yq = yq')"
+  by auto
+
+value "deterministic m_ex_H"
+
+
+subsubsection \<open>Observable\<close>
+
+fun observable :: "('a,'b,'c) fsm \<Rightarrow> bool" where
+  "observable M = (\<forall> t1 \<in> transitions M . \<forall> t2 \<in> transitions M . t_source t1 = t_source t2 \<and> t_input t1 = t_input t2 \<and> t_output t1 = t_output t2 \<longrightarrow> t_target t1 = t_target t2)" 
+
+lemma observable_alt_def : "observable M = (\<forall> q1 x y q1' q1'' . (q1,x,y,q1') \<in> transitions M \<and> (q1,x,y,q1'') \<in> transitions M \<longrightarrow> q1' = q1'')" 
+  by auto
+
+lemma observable_alt_def_h : "observable M = (\<forall> q1 x yq yq' . (yq \<in> h M (q1,x) \<and> yq' \<in> h M (q1,x)) \<longrightarrow> fst yq = fst yq' \<longrightarrow> snd yq = snd yq')"
+  by auto
+
+value "observable m_ex_H"
+
+
+
+subsubsection \<open>Single Input\<close>
+
+
+(* each state has at most one input, but may have none *)
+fun single_input :: "('a,'b,'c) fsm \<Rightarrow> bool" where
+  "single_input M = (\<forall> t1 \<in> transitions M . \<forall> t2 \<in> transitions M . t_source t1 = t_source t2 \<longrightarrow> t_input t1 = t_input t2)" 
+
+
+lemma single_input_alt_def : "single_input M = (\<forall> q1 x x' y y' q1' q1'' . (q1,x,y,q1') \<in> transitions M \<and> (q1,x',y',q1'') \<in> transitions M \<longrightarrow> x = x')"
+  by fastforce
+
+lemma single_input_alt_def_h : "single_input M = (\<forall> q x x' . (h M (q,x) \<noteq> {} \<and> h M (q,x') \<noteq> {}) \<longrightarrow> x = x')"
+  by force
+    
+value "single_input m_ex_H"  
+
+
+
+subsubsection \<open>Output Complete\<close>
+
+fun output_complete :: "('a,'b,'c) fsm \<Rightarrow> bool" where
+  "output_complete M = (\<forall> t \<in> transitions M . \<forall> y \<in> outputs M . \<exists> t' \<in> transitions M . t_source t = t_source t' \<and> t_input t = t_input t' \<and> t_output t' = y)" 
+
+lemma output_complete_alt_def : "output_complete M = (\<forall> q x . (\<exists> y q' . (q,x,y,q') \<in> transitions M) \<longrightarrow> (\<forall> y \<in> (outputs M) . \<exists> q' . (q,x,y,q') \<in> transitions M))" 
+  by force
+
+lemma output_complete_alt_def_h : "output_complete M = (\<forall> q x . h M (q,x) \<noteq> {} \<longrightarrow> (\<forall> y \<in> outputs M . \<exists> q' . (y,q') \<in> h M (q,x)))"
+  by force
+
+value "output_complete m_ex_H"
+
+
+
+subsubsection \<open>Acyclic\<close>
+
+fun acyclic :: "('a,'b,'c) fsm \<Rightarrow> bool" where
+  "acyclic M = (\<forall> p . path M (initial M) p \<longrightarrow> distinct (visited_nodes (initial M) p))"
+
+
+lemma visited_nodes_length : "length (visited_nodes q p) = Suc (length p)" by auto
+
+lemma visited_nodes_take : 
+  "(take (Suc n) (visited_nodes q p)) = (visited_nodes q (take n p))"
+proof (induction p rule: rev_induct)
+  case Nil
+  then show ?case by auto
+next
+  case (snoc x xs)
+  then show ?case by (cases "n \<le> length xs"; auto)
+qed
+
+
+(* very inefficient calculation *)
+lemma acyclic_code[code] : "acyclic M = (\<not>(\<exists> p \<in> (acyclic_paths_up_to_length M (initial M) (size M - 1)) . \<exists> t \<in> transitions M . t_source t = target (initial M) p \<and> t_target t \<in> set (visited_nodes (initial M) p)))"
+proof -
+  have "(\<exists> p \<in> (acyclic_paths_up_to_length M (initial M) (size M - 1)) . \<exists> t \<in> transitions M . t_source t = target (initial M) p \<and> t_target t \<in> set (visited_nodes (initial M) p)) \<Longrightarrow> \<not> FSM.acyclic M"
+  proof -
+    assume "(\<exists> p \<in> (acyclic_paths_up_to_length M (initial M) (size M - 1)) . \<exists> t \<in> transitions M . t_source t = target (initial M) p \<and> t_target t \<in> set (visited_nodes (initial M) p))"
+    then obtain p t where "path M (initial M) p"
+                    and   "distinct (visited_nodes (initial M) p)"
+                    and   "t \<in> transitions M"
+                    and   "t_source t = target (initial M) p" 
+                    and   "t_target t \<in> set (visited_nodes (initial M) p)"
+      unfolding acyclic_paths_set by blast
+    then have "path M (initial M) (p@[t])"
+      by (simp add: path_append_transition) 
+    moreover have "\<not> (distinct (visited_nodes (initial M) (p@[t])))"
+      using \<open>t_target t \<in> set (visited_nodes (initial M) p)\<close> by auto
+    ultimately show "\<not> FSM.acyclic M"
+      by (meson acyclic.elims(2))
+  qed
+  moreover have "\<not> FSM.acyclic M \<Longrightarrow> (\<exists> p \<in> (acyclic_paths_up_to_length M (initial M) (size M - 1)) . \<exists> t \<in> transitions M . t_source t = target (initial M) p \<and> t_target t \<in> set (visited_nodes (initial M) p))"
+  proof -
+    assume "\<not> FSM.acyclic M"
+    then obtain p where "path M (initial M) p"
+                  and   "\<not> distinct (visited_nodes (initial M) p)"
+      by auto
+    then obtain n where "distinct (take (Suc n) (visited_nodes (initial M) p))"
+                  and   "\<not> distinct (take (Suc (Suc n)) (visited_nodes (initial M) p))"
+      using maximal_distinct_prefix by blast
+    then have "distinct (visited_nodes (initial M) (take n p))"
+         and   "\<not> distinct (visited_nodes (initial M)(take (Suc n) p))"
+      unfolding visited_nodes_take by simp+
+
+    then obtain p' t' where *: "take n p = p'"
+                      and   **: "take (Suc n) p = p' @ [t']"
+      by (metis Suc_less_eq \<open>\<not> distinct (visited_nodes (FSM.initial M) p)\<close> le_imp_less_Suc not_less_eq_eq take_all take_hd_drop)
+    
+    have ***: "visited_nodes (FSM.initial M) (p' @ [t']) = (visited_nodes (FSM.initial M) p')@[t_target t']"
+      by auto
+
+    have "path M (initial M) p'"
+      using * \<open>path M (initial M) p\<close>
+      by (metis append_take_drop_id path_prefix)
+    then have "p' \<in> (acyclic_paths_up_to_length M (initial M) (size M - 1))"
+      using \<open>distinct (visited_nodes (initial M) (take n p))\<close>
+      unfolding * acyclic_paths_set by blast
+    moreover have "t' \<in> transitions M \<and> t_source t' = target (initial M) p'"
+      using * ** \<open>path M (initial M) p\<close>
+      by (metis append_take_drop_id path_append_elim path_cons_elim)
+       
+    moreover have "t_target t' \<in> set (visited_nodes (initial M) p')"
+      using \<open>distinct (visited_nodes (initial M) (take n p))\<close> \<open>\<not> distinct (visited_nodes (initial M)(take (Suc n) p))\<close>
+      unfolding * ** *** by auto 
+    ultimately show "(\<exists> p \<in> (acyclic_paths_up_to_length M (initial M) (size M - 1)) . \<exists> t \<in> transitions M . t_source t = target (initial M) p \<and> t_target t \<in> set (visited_nodes (initial M) p))"
+      by blast
+  qed
+  ultimately show ?thesis by blast
+qed
+
+
+value "acyclic m_ex_H"
+
+
+lemma acyclic_alt_def : "acyclic M = finite (L M)"
+proof 
+  show "acyclic M \<Longrightarrow> finite (L M)"
+  proof -
+    assume "acyclic M"
+    then have "{ p . path M (initial M) p} \<subseteq> (acyclic_paths_up_to_length M (initial M) (size M - 1))"
+      unfolding acyclic_paths_set by auto
+    moreover have "finite (acyclic_paths_up_to_length M (initial M) (size M - 1))"
+      unfolding acyclic_paths_up_to_length.simps using paths_finite[of M "initial M" "size M - 1"]
+      by (metis (mono_tags, lifting) Collect_cong \<open>FSM.acyclic M\<close> acyclic.elims(2)) 
+    ultimately have "finite { p . path M (initial M) p}"
+      using finite_subset by blast
+    then show "finite (L M)"
+      unfolding LS.simps by auto
+  qed
+
+  show "finite (L M) \<Longrightarrow> acyclic M"
+  proof (rule ccontr)
+    assume "finite (L M)"
+    assume "\<not> acyclic M"
+    
+    obtain max_io_len where "\<forall>io \<in> L M . length io < max_io_len"
+      using finite_maxlen[OF \<open>finite (L M)\<close>] by blast
+    then have "\<And> p . path M (initial M) p \<Longrightarrow> length p < max_io_len"
+    proof -
+      fix p assume "path M (initial M) p"
+      show "length p < max_io_len"
+      proof (rule ccontr)
+        assume "\<not> length p < max_io_len"
+        then have "\<not> length (p_io p) < max_io_len" by auto
+        moreover have "p_io p \<in> L M"
+          unfolding LS.simps using \<open>path M (initial M) p\<close> by blast
+        ultimately show "False"
+          using \<open>\<forall>io \<in> L M . length io < max_io_len\<close> by blast
+      qed
+    qed
+
+    obtain p where "path M (initial M) p" and "\<not> distinct (visited_nodes (initial M) p)"
+      using \<open>\<not> acyclic M\<close> unfolding acyclic.simps by blast
+    then obtain pL where "path M (initial M) pL" and "max_io_len \<le> length pL"
+      using cyclic_path_pumping[of M p max_io_len] by blast
+    then show "False"
+      using \<open>\<And> p . path M (initial M) p \<Longrightarrow> length p < max_io_len\<close>
+      using not_le by blast 
+  qed
+qed
+
+
+lemma acyclic_finite_paths_from_reachable_node :
+  assumes "acyclic M"
+  and     "path M (initial M) p" 
+  and     "target (initial M) p = q"
+    shows "finite {p . path M q p}"
+proof -
+  from assms have "{ p . path M (initial M) p} \<subseteq> (acyclic_paths_up_to_length M (initial M) (size M - 1))"
+    unfolding acyclic_paths_set by auto
+  moreover have "finite (acyclic_paths_up_to_length M (initial M) (size M - 1))"
+    unfolding acyclic_paths_up_to_length.simps using paths_finite[of M "initial M" "size M - 1"]
+    by (metis (mono_tags, lifting) Collect_cong \<open>FSM.acyclic M\<close> acyclic.elims(2)) 
+  ultimately have "finite { p . path M (initial M) p}"
+    using finite_subset by blast
+
+  show "finite {p . path M q p}"
+  proof (cases "q \<in> nodes M")
+    case True
+        
+    have "image (\<lambda>p' . p@p') {p' . path M q p'} \<subseteq> {p' . path M (initial M) p'}"
+    proof 
+      fix x assume "x \<in> image (\<lambda>p' . p@p') {p' . path M q p'}"
+      then obtain p' where "x = p@p'" and "p' \<in> {p' . path M q p'}"
+        by blast
+      then have "path M q p'" by auto
+      then have "path M (initial M) (p@p')"
+        using path_append[OF \<open>path M (initial M) p\<close>] \<open>target (initial M) p = q\<close> by auto
+      then show "x \<in> {p' . path M (initial M) p'}" using \<open>x = p@p'\<close> by blast
+    qed
+    
+    then have "finite (image (\<lambda>p' . p@p') {p' . path M q p'})"
+      using \<open>finite { p . path M (initial M) p}\<close> finite_subset by auto 
+    show ?thesis using finite_imageD[OF \<open>finite (image (\<lambda>p' . p@p') {p' . path M q p'})\<close>]
+      by (meson inj_onI same_append_eq) 
+  next
+    case False
+    then show ?thesis
+      by (meson not_finite_existsD path_begin_node) 
+  qed
+qed
+
+
+lemma acyclic_paths_from_reachable_nodes :
+  assumes "acyclic M" 
+  and     "path M (initial M) p'" 
+  and     "target (initial M) p' = q"
+  and     "path M q p"
+shows "distinct (visited_nodes q p)"
+proof -
+  have "path M (initial M) (p'@p)"
+    using assms(2,3,4) path_append by metis
+  then have "distinct (visited_nodes (initial M) (p'@p))"
+    using assms(1) unfolding acyclic.simps by blast
+  then have "distinct (initial M # (map t_target p') @ map t_target p)"
+    by auto
+  moreover have "initial M # (map t_target p') @ map t_target p = (butlast (initial M # map t_target p')) @ ((last (initial M # map t_target p')) # map t_target p)"
+    by auto
+  ultimately have "distinct ((last (initial M # map t_target p')) # map t_target p)"
+    by auto
+  then show ?thesis 
+    using \<open>target (initial M) p' = q\<close> unfolding visited_nodes.simps target.simps by simp
+qed
+
+definition LS_acyclic :: "('a,'b,'c) fsm \<Rightarrow> 'a \<Rightarrow> ('b \<times> 'c) list set" where
+  "LS_acyclic M q = {p_io p | p .  path M q p \<and> distinct (visited_nodes q p)}"
+
+lemma LS_acyclic_code[code] : 
+  "LS_acyclic M q = image p_io (acyclic_paths_up_to_length M q (size M - 1))"
+  unfolding acyclic_paths_set LS_acyclic_def by blast
+
+lemma LS_from_LS_acyclic : 
+  assumes "acyclic M" 
+  shows "L M = LS_acyclic M (initial M)"
+proof -
+  obtain pps :: "(('b \<times> 'c) list \<Rightarrow> bool) \<Rightarrow> (('b \<times> 'c) list \<Rightarrow> bool) \<Rightarrow> ('b \<times> 'c) list" where
+    f1: "\<forall>p pa. (\<not> p (pps pa p)) = pa (pps pa p) \<or> Collect p = Collect pa"
+    by (metis (no_types) Collect_cong)
+  have "\<forall>ps. \<not> path M (FSM.initial M) ps \<or> distinct (visited_nodes (FSM.initial M) ps)"
+    using acyclic.simps assms by blast
+  then have "(\<nexists>ps. pps (\<lambda>ps. \<exists>psa. ps = p_io psa \<and> path M (FSM.initial M) psa) (\<lambda>ps. \<exists>psa. ps = p_io psa \<and> path M (FSM.initial M) psa \<and> distinct (visited_nodes (FSM.initial M) psa)) = p_io ps \<and> path M (FSM.initial M) ps \<and> distinct (visited_nodes (FSM.initial M) ps)) \<noteq> (\<exists>ps. pps (\<lambda>ps. \<exists>psa. ps = p_io psa \<and> path M (FSM.initial M) psa) (\<lambda>ps. \<exists>psa. ps = p_io psa \<and> path M (FSM.initial M) psa \<and> distinct (visited_nodes (FSM.initial M) psa)) = p_io ps \<and> path M (FSM.initial M) ps)"
+    by blast
+  then have "{p_io ps |ps. path M (FSM.initial M) ps \<and> distinct (visited_nodes (FSM.initial M) ps)} = {p_io ps |ps. path M (FSM.initial M) ps}"
+    using f1 by (meson \<open>\<forall>ps. \<not> path M (FSM.initial M) ps \<or> distinct (visited_nodes (FSM.initial M) ps)\<close>) 
+  then show ?thesis
+    by (simp add: LS_acyclic_def)
+qed
+
+
+
+lemma cyclic_cycle :
+  assumes "\<not> acyclic M"
+  shows "\<exists> q p . path M q p \<and> p \<noteq> [] \<and> target q p = q" 
+proof -
+  from \<open>\<not> acyclic M\<close> obtain p t where "path M (initial M) (p@[t])" and "\<not>distinct (visited_nodes (initial M) (p@[t]))"
+    by (metis (no_types, hide_lams) Nil_is_append_conv acyclic.simps append_take_drop_id maximal_distinct_prefix rev_exhaust visited_nodes_take)
+     
+
+  show ?thesis
+  proof (cases "initial M \<in> set (map t_target (p@[t]))")
+    case True
+    then obtain i where "last (take i (map t_target (p@[t]))) = initial M" and "i \<le> length (map t_target (p@[t]))" and "0 < i"
+      using list_contains_last_take by metis
+
+    let ?p = "take i (p@[t])"
+    have "path M (initial M) (?p@(drop i (p@[t])))" 
+      using \<open>path M (initial M) (p@[t])\<close>
+      by (metis append_take_drop_id)  
+    then have "path M (initial M) ?p" by auto
+    moreover have "?p \<noteq> []" using \<open>0 < i\<close> by auto
+    moreover have "target (initial M) ?p = initial M"
+      using \<open>last (take i (map t_target (p@[t]))) = initial M\<close> unfolding target.simps visited_nodes.simps
+      by (metis (no_types, lifting) calculation(2) last_ConsR list.map_disc_iff take_map) 
+    ultimately show ?thesis by blast
+  next
+    case False
+    then have "\<not> distinct (map t_target (p@[t]))"
+      using \<open>\<not>distinct (visited_nodes (initial M) (p@[t]))\<close> unfolding visited_nodes.simps by auto
+    then obtain i j where "i < j" and "j < length (map t_target (p@[t]))" and "(map t_target (p@[t])) ! i = (map t_target (p@[t])) ! j"
+      using non_distinct_repetition_indices by blast
+
+    let ?pre_i = "take (Suc i) (p@[t])"
+    let ?p = "take ((Suc j)-(Suc i)) (drop (Suc i) (p@[t]))"
+    let ?post_j = "drop ((Suc j)-(Suc i)) (drop (Suc i) (p@[t]))"
+
+    have "p@[t] = ?pre_i @ ?p @ ?post_j"
+      using \<open>i < j\<close> \<open>j < length (map t_target (p@[t]))\<close>
+      by (metis append_take_drop_id) 
+    then have "path M (target (initial M) ?pre_i) ?p" 
+      using \<open>path M (initial M) (p@[t])\<close>
+      by (metis path_prefix path_suffix) 
+
+    have "?p \<noteq> []"
+      using \<open>i < j\<close> \<open>j < length (map t_target (p@[t]))\<close> by auto
+
+    have "i < length (map t_target (p@[t]))"
+      using \<open>i < j\<close> \<open>j < length (map t_target (p@[t]))\<close> by auto
+    have "(target (initial M) ?pre_i) = (map t_target (p@[t])) ! i"
+      unfolding target.simps visited_nodes.simps  
+      using take_last_index[OF \<open>i < length (map t_target (p@[t]))\<close>]
+      by (metis (no_types, lifting) \<open>i < length (map t_target (p @ [t]))\<close> last_ConsR snoc_eq_iff_butlast take_Suc_conv_app_nth take_map) 
+    
+    have "?pre_i@?p = take (Suc j) (p@[t])"
+      by (metis (no_types) \<open>i < j\<close> add_Suc add_diff_cancel_left' less_SucI less_imp_Suc_add take_add)
+    moreover have "(target (initial M) (take (Suc j) (p@[t]))) = (map t_target (p@[t])) ! j"
+      unfolding target.simps visited_nodes.simps  
+      using take_last_index[OF \<open>j < length (map t_target (p@[t]))\<close>]
+      by (metis (no_types, lifting) \<open>j < length (map t_target (p @ [t]))\<close> last_ConsR snoc_eq_iff_butlast take_Suc_conv_app_nth take_map) 
+    ultimately have "(target (initial M) (?pre_i@?p)) = (map t_target (p@[t])) ! j"
+      by auto
+    then have "(target (initial M) (?pre_i@?p)) = (map t_target (p@[t])) ! i"
+      using \<open>(map t_target (p@[t])) ! i = (map t_target (p@[t])) ! j\<close> by simp
+    moreover have "(target (initial M) (?pre_i@?p)) = (target (target (initial M) ?pre_i) ?p)"
+      unfolding target.simps visited_nodes.simps last.simps by auto
+    ultimately have "(target (target (initial M) ?pre_i) ?p) = (map t_target (p@[t])) ! i"
+      by auto
+    then have "(target (target (initial M) ?pre_i) ?p) = (target (initial M) ?pre_i)"
+      using \<open>(target (initial M) ?pre_i) = (map t_target (p@[t])) ! i\<close> by auto
+
+    show ?thesis
+      using \<open>path M (target (initial M) ?pre_i) ?p\<close> \<open>?p \<noteq> []\<close> \<open>(target (target (initial M) ?pre_i) ?p) = (target (initial M) ?pre_i)\<close>
+      by blast
+  qed
+qed
+
+
+lemma cyclic_cycle_rev :
+  fixes M :: "('a,'b,'c) fsm"
+  assumes "path M (initial M) p'"
+  and     "target (initial M) p' = q" 
+  and     "path M q p"
+  and     "p \<noteq> []"
+  and     "target q p = q"
+shows "\<not> acyclic M"
+  using assms unfolding acyclic.simps target.simps visited_nodes.simps
+  using distinct.simps(2) by fastforce
+
+lemma acyclic_initial :
+  assumes "acyclic M"
+  shows "\<not> (\<exists> t \<in> transitions M . t_target t = initial M \<and> (\<exists> p . path M (initial M) p \<and> target (initial M) p = t_source t))"
+  by (metis append_Cons assms cyclic_cycle_rev list.distinct(1) path.simps path_append path_append_transition_elim(3) single_transition_path) 
+
+lemma cyclic_path_shift : 
+  assumes "path M q p"
+  and     "target q p = q"
+shows "path M (target q (take i p)) ((drop i p) @ (take i p))"
+  and "target (target q (take i p)) ((drop i p) @ (take i p)) = (target q (take i p))"
+proof -
+  show "path M (target q (take i p)) ((drop i p) @ (take i p))"
+    by (metis append_take_drop_id assms(1) assms(2) path_append path_append_elim path_append_target)
+  show "target (target q (take i p)) ((drop i p) @ (take i p)) = (target q (take i p))"
+    by (metis append_take_drop_id assms(2) path_append_target)
+qed
+
+
+lemma cyclic_path_transition_nodes_property :
+  assumes "\<exists> t \<in> set p . P (t_source t)"
+  and     "\<forall> t \<in> set p . P (t_source t) \<longrightarrow> P (t_target t)"
+  and     "path M q p"
+  and     "target q p = q"
+shows "\<forall> t \<in> set p . P (t_source t)"
+  and "\<forall> t \<in> set p . P (t_target t)"
+proof -
+  obtain t0 where "t0 \<in> set p" and "P (t_source t0)"
+    using assms(1) by blast
+  then obtain i where "i < length p" and "p ! i = t0"
+    by (meson in_set_conv_nth)
+
+  let ?p = "(drop i p @ take i p)"
+  have "path M (target q (take i p)) ?p"
+    using cyclic_path_shift(1)[OF assms(3,4), of i] by assumption
+  
+  have "set ?p = set p"
+  proof -
+    have "set ?p = set (take i p @ drop i p)" 
+      using list_set_sym by metis
+    then show ?thesis by auto
+  qed
+  then have "\<And> t . t \<in> set ?p \<Longrightarrow> P (t_source t) \<Longrightarrow> P (t_target t)"
+    using assms(2) by blast
+  
+  have "\<And> j . j < length ?p \<Longrightarrow> P (t_source (?p ! j))"
+  proof -
+    fix j assume "j < length ?p"
+    then show "P (t_source (?p ! j))"
+    proof (induction j)
+      case 0
+      then show ?case 
+        using \<open>p ! i = t0\<close> \<open>P (t_source t0)\<close>
+        by (metis \<open>i < length p\<close> drop_eq_Nil hd_append2 hd_conv_nth hd_drop_conv_nth leD length_greater_0_conv)  
+    next
+      case (Suc j)
+      then have "P (t_source (?p ! j))"
+        by auto
+      then have "P (t_target (?p ! j))"
+        using Suc.prems \<open>\<And> t . t \<in> set ?p \<Longrightarrow> P (t_source t) \<Longrightarrow> P (t_target t)\<close>[of "?p ! j"]
+        using Suc_lessD nth_mem by blast 
+      moreover have "t_target (?p ! j) = t_source (?p ! (Suc j))"
+        using path_source_target_index[OF Suc.prems \<open>path M (target q (take i p)) ?p\<close>] by assumption
+      ultimately show ?case 
+        using \<open>\<And> t . t \<in> set ?p \<Longrightarrow> P (t_source t) \<Longrightarrow> P (t_target t)\<close>[of "?p ! j"]
+        by simp
+    qed
+  qed
+  then have "\<forall> t \<in> set ?p . P (t_source t)"
+    by (metis in_set_conv_nth)
+  then show "\<forall> t \<in> set p . P (t_source t)"
+    using \<open>set ?p = set p\<close> by blast
+  then show "\<forall> t \<in> set p . P (t_target t)"
+    using assms(2) by blast
+qed
+
+
+lemma cycle_incoming_transition_ex :
+  assumes "path M q p"
+  and     "p \<noteq> []"
+  and     "target q p = q"
+  and     "t \<in> set p"
+shows "\<exists> tI \<in> set p . t_target tI = t_source t"
+proof -
+  obtain i where "i < length p" and "p ! i = t"
+    using assms(4) by (meson in_set_conv_nth)
+
+  let ?p = "(drop i p @ take i p)"
+  have "path M (target q (take i p)) ?p"
+  and  "target (target q (take i p)) ?p = target q (take i p)"
+    using cyclic_path_shift[OF assms(1,3), of i] by linarith+
+
+  have "p = (take i p @ drop i p)" by auto
+  then have "path M (target q (take i p)) (drop i p)" 
+    using path_suffix assms(1) by metis
+  moreover have "t = hd (drop i p)"
+    using \<open>i < length p\<close> \<open>p ! i = t\<close>
+    by (simp add: hd_drop_conv_nth) 
+  ultimately have "path M (target q (take i p)) [t]"
+    by (metis \<open>i < length p\<close> append_take_drop_id assms(1) path_append_elim take_hd_drop)
+  then have "t_source t = (target q (take i p))"
+    by auto  
+  moreover have "t_target (last ?p) = (target q (take i p))"
+    using \<open>path M (target q (take i p)) ?p\<close> \<open>target (target q (take i p)) ?p = target q (take i p)\<close> assms(2)
+    unfolding target.simps visited_nodes.simps last.simps
+  proof -
+    assume a1: "(if map t_target (drop i p @ take i p) = [] then if map t_target (take i p) = [] then q else last (map t_target (take i p)) else last (map t_target (drop i p @ take i p))) = (if map t_target (take i p) = [] then q else last (map t_target (take i p)))"
+    have "drop i p @ take i p \<noteq> [] \<and> map t_target (drop i p @ take i p) \<noteq> []"
+      using \<open>p \<noteq> []\<close> by fastforce
+    moreover
+    { assume "map t_target (take i p) \<noteq> [] \<and> map t_target (drop i p @ take i p) \<noteq> []"
+      then have "t_target (last (drop i p @ take i p)) = (if map t_target (take i p) = [] then q else last (map t_target (take i p)))"
+        by (simp add: last_map) }
+    ultimately show "t_target (last (drop i p @ take i p)) = (if map t_target (take i p) = [] then q else last (map t_target (take i p)))"
+      using a1 by (metis (no_types) last_map)
+  qed
+    
+  
+  moreover have "set ?p = set p"
+  proof -
+    have "set ?p = set (take i p @ drop i p)" 
+      using list_set_sym by metis
+    then show ?thesis by auto
+  qed
+
+  ultimately show ?thesis
+    by (metis \<open>i < length p\<close> append_is_Nil_conv drop_eq_Nil last_in_set leD) 
+qed
+
+
+subsubsection \<open>Deadlock Nodes\<close>
+
+fun deadlock_state :: "('a,'b,'c) fsm \<Rightarrow> 'a \<Rightarrow> bool" where 
+  "deadlock_state M q = (\<not>(\<exists> t \<in> transitions M . t_source t = q))"
+
+lemma deadlock_state_alt_def : "deadlock_state M q = (LS M q \<subseteq> {[]})" 
+proof 
+  show "deadlock_state M q \<Longrightarrow> LS M q \<subseteq> {[]}" 
+  proof -
+    assume "deadlock_state M q"
+    moreover have "\<And> p . deadlock_state M q \<Longrightarrow> path M q p \<Longrightarrow> p = []"
+      unfolding deadlock_state.simps by (metis path.cases) 
+    ultimately show "LS M q \<subseteq> {[]}"
+      unfolding LS.simps by blast
+  qed
+  show "LS M q \<subseteq> {[]} \<Longrightarrow> deadlock_state M q"
+    unfolding LS.simps deadlock_state.simps using path.cases[of M q] by blast
+qed
+
+lemma deadlock_state_alt_def_h : "deadlock_state M q = (\<forall> x \<in> inputs M . h M (q,x) = {})" 
+  unfolding deadlock_state.simps h.simps 
+  using fsm_transition_input by force
+
+
+lemma acyclic_deadlock_states :
+  assumes "acyclic M"
+  shows "\<exists> q \<in> nodes M . deadlock_state M q"
+proof (rule ccontr)
+  assume "\<not> (\<exists>q\<in>nodes M. deadlock_state M q)"
+  then have *: "\<And> q . q \<in> nodes M \<Longrightarrow> (\<exists> t \<in> transitions M . t_source t = q)"
+    unfolding deadlock_state.simps by blast
+
+  let ?p = "arg_max_on length {p. path M (initial M) p}"
+  
+
+  have "finite {p. path M (initial M) p}" 
+    by (metis Collect_cong acyclic_finite_paths_from_reachable_node assms eq_Nil_appendI fsm_initial nil path_append path_append_elim) 
+    
+  moreover have "{p. path M (initial M) p} \<noteq> {}" 
+    by auto
+  ultimately obtain p where "path M (initial M) p" and "\<And> p' . path M (initial M) p' \<Longrightarrow> length p' \<le> length p" 
+    using max_length_elem
+    by (metis mem_Collect_eq not_le_imp_less)
+
+  then obtain t where "t \<in> transitions M" and "t_source t = target (initial M) p"
+    using * path_target_is_node by metis
+
+  then have "path M (initial M) (p@[t])"
+    using \<open>path M (initial M) p\<close>
+    by (simp add: path_append_transition)
+
+  then show "False"
+    using \<open>\<And> p' . path M (initial M) p' \<Longrightarrow> length p' \<le> length p\<close>
+    by (metis impossible_Cons length_rotate1 rotate1.simps(2)) 
+qed
+
+lemma deadlock_prefix :
+  assumes "path M q p"
+  and     "t \<in> set (butlast p)"
+shows "\<not> (deadlock_state M (t_target t))"
+  using assms proof (induction p rule: rev_induct)
+  case Nil
+  then show ?case by auto
+next
+  case (snoc t' p')
+  
+  show ?case proof (cases "t \<in> set (butlast p')")
+    case True
+    show ?thesis 
+      using snoc.IH[OF _ True] snoc.prems(1)
+      by blast 
+  next
+    case False
+    then have "p' = (butlast p')@[t]"
+      using snoc.prems(2) by (metis append_butlast_last_id append_self_conv2 butlast_snoc in_set_butlast_appendI list_prefix_elem set_ConsD)
+    then have "path M q ((butlast p'@[t])@[t'])"
+      using snoc.prems(1)
+      by auto 
+    
+    have "t' \<in> transitions M" and "t_source t' = target q (butlast p'@[t])"
+      using path_suffix[OF \<open>path M q ((butlast p'@[t])@[t'])\<close>]
+      by auto
+    then have "t' \<in> transitions M \<and> t_source t' = t_target t"
+      unfolding target.simps visited_nodes.simps by auto
+    then show ?thesis 
+      unfolding deadlock_state.simps using \<open>t' \<in> transitions M\<close> by blast
+  qed
+qed
+
+
+subsubsection \<open>Other\<close>
+
+fun completed_path :: "('a,'b,'c) fsm \<Rightarrow> 'a \<Rightarrow> ('a,'b,'c) path \<Rightarrow> bool" where
+  "completed_path M q p = deadlock_state M (target q p)"
+
+fun minimal :: "('a,'b,'c) fsm \<Rightarrow> bool" where
+  "minimal M = (\<forall> q \<in> nodes M . \<forall> q' \<in> nodes M . q \<noteq> q' \<longrightarrow> LS M q \<noteq> LS M q')"
+
+definition retains_outputs_for_states_and_inputs :: "('a,'b,'c) fsm \<Rightarrow> ('a,'b,'c) fsm \<Rightarrow> bool" where
+  "retains_outputs_for_states_and_inputs M S = (\<forall> tS \<in> transitions S . \<forall> tM \<in> transitions M . (t_source tS = t_source tM \<and> t_input tS = t_input tM) \<longrightarrow> tM \<in> transitions S)"
+
 
 
 
